rustfrontend/BorrowCheckSound.v
@@ -1,0 +1,759 @@
+Require Import Coqlib .
+Require Import Errors Maps.
+Require Import Values.
+Require Import Integers.
+Require Import AST.
+Require Import Memory.
+Require Import Events.
+Require Import Globalenvs Linking.
+Require Import Smallstep SmallstepLinking SmallstepLinkingSafe.
+Require Import LanguageInterface CKLR Invariant.
+Require Import Rusttypes Rustlight Rustlightown.
+Require Import RustOp RustIR RustIRcfg Rusttyping.
+Require Import Errors.
+Require Import InitDomain InitAnalysis.
+Require Import RustIRown MoveChecking.
+Require Import MoveCheckingFootprint MoveCheckingDomain.
+Require Import StkBorPermission RustIRbor.
+Require Import RegionLiveness BorrowCheckDomain.
+Require Import BorrowCheckPolonius BorrowCheck.
+Require Import Wfsimpl.
+(* use free_list related lemmas *)
+Require SimplLocalsproof.
+
+Import ListNotations.
+Local Open Scope error_monad_scope.
+Local Open Scope inv_scope.
+
+
+Section BORROW_CHECK.
+
+Variable prog: program.
+Variable w: rs_own_world.
+Variable se: Genv.symtbl.
+Hypothesis VALIDSE: Genv.valid_for (erase_program prog) se.
+Let L := semantics prog se.
+Let ge := globalenv se prog.
+
+(* composite environment *)
+Let ce := ge.(genv_cenv).
+
+Definition mod_sg := match w with
+                    | rsw sg _ _ _ => sg
+                    end.
+
+Let wt_state := wt_state prog se mod_sg.
+
+(* split move_check_program_spec into the following hypotheses to simplify the proof *)
+Hypothesis CONSISTENT: composite_env_consistent ce.
+
+Hypothesis COMP_RANGE: forall id co, ce ! id = Some co -> co_sizeof co <= Ptrofs.max_unsigned.
+Hypothesis COMP_LEN: forall id co, ce ! id = Some co -> list_length_z (co_members co) <= Int.max_unsigned.
+Hypothesis COMP_NOREP: forall id co, ce ! id = Some co -> list_norepet (name_members (co_members co)).
+(* Hypothesis FUN_CHECK:  forall id fd, *)
+(*     In (id, Gfun fd) prog.(prog_defs) -> *)
+(*     move_check_fundef_spec ce fd. *)
+
+(* Result of the init analysis and the result of the move checking *)
+
+Let INIT_AN : Type := (PMap.t IM.t * PMap.t IM.t * PathsMap.t).
+
+Let move_check_stmt (ae: INIT_AN) body cfg s ts := match_stmt get_init_info ae (move_check_stmt ce) (check_cond_expr ce) body cfg s ts.
+
+(* Result of the loans-flow analysis and the result of the borrow
+checking *)
+
+Let LOANS_AN : Type := (PMap.t RegionSet.t * PMap.t LoansEnv.t).
+
+Let borrow_check_stmt (ae: LOANS_AN) regs f cfg s ts := match_stmt (get_borck_result regs f cfg) ae (borrow_check_stmt f) borrow_check_cond_expr f.(fn_body) cfg s ts.
+
+(*********** Properties for the evaluation of place and expression ****************** *)
+
+Lemma sizeof_in_range: forall ty,
+    valid_type ty = true ->
+    sizeof ce ty <= Ptrofs.max_unsigned.
+Proof.
+  destruct ty; simpl; rewrite maxv; try lia.
+  destruct i; lia.
+  destruct f; lia.
+  destruct Archi.ptr64; lia.
+  destruct Archi.ptr64; lia.
+  congruence.
+  destruct (ce ! i) eqn: A; try lia. 
+  generalize (COMP_RANGE i c A). rewrite maxv. auto.
+  destruct (ce ! i) eqn: A; try lia. 
+  generalize (COMP_RANGE i c A). rewrite maxv. auto.
+Qed.
+
+
+(* The locations evaluated by get_loc_footprint_map and eval_place are
+the same. To support reference, we should provide that regions in p
+are live and the invariant for the loans environment and stacked
+borrow memory *)
+Lemma eval_place_get_loc_footprint_map_equal: forall m le p fpm fp b1 ofs1 b2 ofs2 own stk1 stk2 af
+    (GFP: get_loc_footprint_map le (path_of_place p) fpm = Some (b1, ofs1, fp))
+    (WT: wt_place le ce p)
+    (WFENV: wf_env fpm ce m le)
+    (EVAL: eval_place ce le m stk1 p b2 ofs2 stk2 af)
+    (MM: mmatch fpm ce m le own)
+    (DOM: dominators_is_init own p = true),
+    b1 = b2
+    /\ ofs1 = Ptrofs.unsigned ofs2
+    (* It is used to strengthen this lemma *)
+    /\ wt_footprint ce (typeof_place p) fp
+    /\ ofs1 + sizeof ce (typeof_place p) <= Ptrofs.max_unsigned.
+Proof.
+  induction p; intros.
+  - inv EVAL. simpl in GFP. rewrite H5 in GFP.
+    destruct (fpm ! i) eqn: FP; try congruence. inv GFP.
+    repeat apply conj; auto.
+    simpl. exploit wf_env_footprint; eauto.
+    intros (fp0 & A1 & A2). rewrite FP in A1. inv A1. auto.
+    simpl. inv WT. eapply sizeof_in_range. auto.
+  - inv EVAL. simpl in GFP. destruct (path_of_place p) eqn: POP.
+    exploit get_loc_footprint_map_app_inv. eauto.
+    intros (b3 & ofs3 & fp3 & G1 & G2).
+    exploit IHp. 1-6: eauto. inv WT. eauto.
+    intros (A1 & A2 & A3 & A4). subst.
+    simpl in G2. destruct fp3; try congruence.
+    destruct (find_fields i fpl) eqn: FIND; try congruence. repeat destruct p0.
+    inv G2. inv A3. rewrite H3 in H0. inv H0.
+    exploit find_fields_some. eauto. intros (B1 & B2). subst.
+    exploit WT2. eauto.
+    intros (fty & C1 & C2 & C3).
+    rewrite H8 in CO. inv CO.
+    rewrite H9 in C2. inv C2.
+    (* some range properties *)
+    rewrite H3 in *. simpl in A4. rewrite H8 in A4.
+    exploit field_offset_in_max_range1. 1-5: eauto.
+    intros (R1 & R2 & R3).
+    (* some rewrite *)
+    inv WT. rewrite H3 in WT3. inv WT3.
+    rewrite H8 in WT4. inv WT4.
+    rewrite C1 in WT5. inv WT5. 
+    repeat apply conj; auto.
+    rewrite Ptrofs.add_unsigned; auto.
+    (** range proof obligation *)
+    rewrite !Ptrofs.unsigned_repr; auto.
+    rewrite !Ptrofs.unsigned_repr; auto.        
+  - inv EVAL. inv WT. destruct (typeof_place p) eqn: PTY; simpl in WT2; try congruence.
+    (* Tbox *)
+    + inv WT2. inv H2; simpl in *; try congruence. inv H.
+      destruct (path_of_place p) eqn: POP. 
+      exploit get_loc_footprint_map_app_inv; eauto.
+      intros (b3 & ofs3 & fp3 & G1 & G2).
+      unfold dominators_is_init in DOM. simpl in DOM.
+      eapply andb_true_iff in DOM. destruct DOM as (D1 & D2).
+      exploit IHp; eauto.
+      intros (A1 & A2 & A3 & A4). subst.
+      simpl in G2. destruct fp3; try congruence. inv G2.
+      inv A3.
+      exploit MM. erewrite POP. eauto. auto. intros (BM & FULL).
+      inv BM. rewrite H0 in LOAD. inv LOAD.
+      repeat apply conj; auto. lia.
+    (** TODO: reference  *)
+    + admit.
+    (* simpl. eapply sizeof_in_range; eauto. *)
+  - inv EVAL. simpl in GFP. destruct (path_of_place p) eqn: POP.
+    exploit get_loc_footprint_map_app_inv; eauto.
+    intros (b3 & ofs3 & fp3 & G1 & G2).
+    unfold dominators_is_init in *. simpl in DOM.
+    eapply andb_true_iff in DOM. destruct DOM as (A & B).
+      assert (DOM1: dominators_is_init own p = true).
+    { destruct p; simpl in *; auto.
+      eapply andb_true_iff. auto. }
+    exploit IHp; eauto. inv WT. eauto.
+    intros (A1 & A2 & A3 & A4). subst.
+    simpl in G2. destruct fp3; try congruence. rewrite H3 in G2.
+    destruct ident_eq in G2; try congruence.
+    destruct List.list_eq_dec in G2; try congruence.
+    destruct ident_eq in G2; try congruence. inv G2.
+    rewrite H3 in A3. inv A3.
+    rewrite H4 in CO. inv CO.
+    rewrite H11 in FOFS. inv FOFS.
+    (* some range properties *)
+    rewrite H3 in *. simpl in A4. rewrite H4 in A4.
+    exploit variant_field_offset_in_max_range1. 1-5: eauto.
+    intros (R1 & R2 & R3).
+    (* some rewrite *)
+    inv WT. rewrite H3 in WT2. inv WT2.
+    rewrite H4 in WT3. inv WT3.
+    repeat apply conj; auto.
+    rewrite Ptrofs.add_unsigned.
+    (** range proof obligation *)
+    rewrite !Ptrofs.unsigned_repr; auto.
+    rewrite !Ptrofs.unsigned_repr; auto.
+    exploit valid_owner_place_footprint. erewrite POP. eauto. eauto.
+    intros (fp' & ofs' & ofs1 & G2 & VFP & OFS).
+    exploit MM. eapply G2. auto.
+    intros (BM' & FULL').
+    assert (BM1: bmatch ce m b1 (Ptrofs.unsigned ofs) (fp_enum id orgs tag0 fid ofs0 fp)).
+    { rewrite OFS. eapply valid_owner_bmatch. eauto. eauto. }
+    inv BM1.
+    simpl in H5. rewrite H5 in TAG0. inv TAG0.
+    rewrite Int.unsigned_repr in H10. rewrite H10 in TAG. inv TAG.
+    simpl. auto.
+    (* tag is in range *)
+    generalize (list_nth_z_range _ _ TAG).
+    generalize (COMP_LEN id co H4). lia.
+    rewrite FTY in WT4. inv WT4.
+    auto.
+Admitted.
+
+
+(* This lemma is used to state that the location of a place is
+unchanged if the memory location in [bs] is unchanged. [bs] is the
+location of the dominator of [p]. It is used to prove the soundness of
+enum assignment where we need to prove that the results of the
+evaluation of p are the same *)
+Lemma eval_place_footprint_unchanged: forall p m b1 b2 ofs1 ofs2 fpm own le fp,
+    get_loc_footprint_map le (path_of_place p) fpm = Some (b1, ofs1, fp) ->
+    eval_place ce le m p b2 ofs2 ->
+    mmatch fpm ce m le own ->
+    dominators_is_init own p = true ->
+    list_norepet (footprint_of_env le ++ flat_fp_map fpm) ->
+    (* These premises are used to reuse eval_place_get_loc_footprint_map_equal *)
+    wf_env fpm ce m le ->
+    wt_place le ce p ->
+    exists bs,
+      (* We have to consider that we cannot change the location of the
+      tag field if p is an enum, very difficult. But we can just
+      ignore the changing in b2 because changing the tag does not
+      affect the field offset *)
+      (* (forall m' b3 ofs3, Mem.unchanged_on (fun b' ofs' => In b' bs) m m' -> *)
+      (*                eval_place ce le m' p b3 ofs3 -> *)
+      (*                b2 = b3 /\ ofs2 = ofs3) *)
+      (forall m', Mem.unchanged_on (fun b' ofs' => In b' bs \/ (b' = b2 /\ ~ ((Ptrofs.unsigned ofs2 <= ofs' < Ptrofs.unsigned ofs2 + sizeof ce (typeof_place p))))) m m' ->
+             eval_place ce le m' p b2 ofs2)
+      /\ list_norepet bs
+      /\ incl bs (footprint_of_env le ++ flat_fp_map fpm)
+      /\ list_disjoint bs (b2 :: footprint_flat fp).
+      (* /\ Ptrofs.unsigned ofs + sizeof ce (typeof_place p) <= Ptrofs.max_unsigned. *)
+Proof.
+  induction p; intros until fp; intros GFP PADDR MM DOM NOREP WFENV WTP.
+  - inv PADDR. simpl in *.
+    rewrite H3 in GFP.
+    destruct (fpm!i) eqn: A; try congruence.
+    inv GFP.
+    exists nil. repeat apply conj.
+    + intros. econstructor; eauto.
+    + constructor.
+    + eapply incl_nil_l.
+    + red. intros. inv H.
+  - exploit eval_place_get_loc_footprint_map_equal; eauto.
+    intros (A1 & A2 & A3 & A4). subst.
+    inv PADDR. simpl in *.
+    destruct (path_of_place p) eqn: POP.
+    exploit get_loc_footprint_map_app_inv; eauto.
+    intros (b1 & ofs1 & fp1 & GFP1 & GFP2). simpl in GFP2.
+    destr_fp_field fp1 GFP2. inv GFP2.
+    inv WTP.
+    (* some rewrite *)
+    rewrite H3 in WT2. inv WT2.
+    rewrite H6 in WT3. inv WT3.
+    exploit IHp; eauto.
+    intros (bs & UNC & NOREP1 & INCL & DIS).
+    (** FIXME: range proof with very bad structure *)
+    exploit eval_place_get_loc_footprint_map_equal. rewrite POP.
+    all: eauto.
+    intros (C1 & C2 & C3 & C4). subst.
+    exploit field_offset_in_range_eq; eauto.
+    rewrite <- H3. eauto. intros (OFSEQ & R1 & R2).
+    exists bs. repeat apply conj; eauto.
+    + intros. econstructor; eauto.
+      eapply UNC. eapply Mem.unchanged_on_implies; eauto.
+      simpl. intros. destruct H0; auto.
+      destruct H0; subst.
+      right. split; auto.
+      intro. eapply H5. rewrite H1 in H0.
+      (* range proof *)
+      rewrite OFSEQ in *. rewrite H3. lia.
+    + red. intros. eapply DIS; auto.
+      inv H0. simpl. auto.
+      eapply in_cons. simpl. eapply in_flat_map; eauto.
+  - exploit eval_place_get_loc_footprint_map_equal; eauto.
+    intros (A1 & A2 & A3 & A4). subst.
+    inv PADDR. simpl in *.
+    destruct (path_of_place p) eqn: POP.
+    exploit get_loc_footprint_map_app_inv; eauto.
+    intros (b1 & ofs1 & fp1 & GFP1 & GFP2). simpl in GFP2.
+    destruct fp1; try congruence. inv GFP2.
+    assert (DOM1: dominators_is_init own p = true).
+    { unfold dominators_is_init in DOM. simpl in DOM.
+      eapply andb_true_iff in DOM. destruct DOM. auto. }
+    inv WTP.
+    exploit IHp; eauto.
+    intros (bs & UNC & NOREP1 & INCL & DIS).
+    exists (l :: bs).
+    exploit eval_place_get_loc_footprint_map_equal; eauto.
+    rewrite POP. eauto.
+    intros (D1 & D2 & D3 & D4). subst.
+    repeat apply conj; eauto.
+    + intros.
+      exploit type_deref_some; eauto. intros PTY.
+      rewrite PTY in *.
+      inv H4; simpl in *; try congruence.      
+      econstructor. eapply UNC.
+      eapply Mem.unchanged_on_implies; eauto.
+      simpl. intros.
+      destruct H4; auto. destruct H4; subst. auto.
+      rewrite PTY in *.
+      eapply deref_loc_value; eauto.
+      eapply Mem.load_unchanged_on; eauto.
+      simpl. intros. auto.
+    + econstructor; auto.
+      intro. eapply DIS; eauto. simpl. auto.
+    + eapply incl_cons; auto.
+      eapply get_loc_footprint_map_in_range; eauto.
+    + red. intros.
+      eapply list_norepet_app in NOREP as (N1 & N2 & N3).
+      inv H.
+      * exploit get_loc_footprint_map_norepet; eauto.
+        intros (E1 & E2). simpl in *.
+        inv H0.
+        -- intro. eapply E2. auto.
+        -- intro. eapply E2. subst. auto.
+      * intro. subst. eapply DIS; eauto.
+        simpl. eauto.
+  - exploit eval_place_get_loc_footprint_map_equal; eauto.
+    intros (A1 & A2 & A3 & A4). subst.
+    inv PADDR. simpl in *.
+    destruct (path_of_place p) eqn: POP.
+    exploit get_loc_footprint_map_app_inv; eauto.
+    intros (b1 & ofs1 & fp1 & GFP1 & GFP2). simpl in GFP2.
+    rewrite H3 in GFP2.
+    destruct fp1; try congruence.
+    destruct ident_eq; try congruence; destruct list_eq_dec; try congruence; destruct ident_eq;  try congruence; subst. inv GFP2.
+    inv WTP.
+    (* some rewrite *)
+    rewrite H3 in WT2. inv WT2.
+    rewrite H4 in WT3. inv WT3.
+    assert (DOM1: dominators_is_init own p = true).
+    { unfold dominators_is_init in *. simpl in DOM.
+      eapply andb_true_iff in DOM. destruct DOM as (A & B).
+      destruct p; simpl in *; auto.
+      eapply andb_true_iff. auto. }
+    exploit IHp; eauto.
+    intros (bs & UNC & NOREP1 & INCL & DIS).
+    exists bs. repeat apply conj; eauto.
+    + intros.
+      (** FIXME: range proof with very bad structure *)
+      exploit eval_place_get_loc_footprint_map_equal. rewrite POP.
+      all: eauto.
+      intros (C1 & C2 & C3 & C4). subst.
+      exploit variant_field_offset_in_range_eq; eauto.
+      rewrite <- H3. eauto. intros (OFSEQ & R1 & R2 & R3).      
+      econstructor; eauto.
+      * eapply UNC. eapply Mem.unchanged_on_implies; eauto.
+        simpl. intros.
+        destruct H0; auto.
+        destruct H0; subst; auto.
+        right. split; auto.
+        intro. eapply H7.
+        rewrite OFSEQ in *. rewrite H1 in *. rewrite H3. lia.
+      * eapply Mem.load_unchanged_on; eauto.
+        simpl. intros. right. split; auto.
+        rewrite H1. rewrite OFSEQ. lia.
+Qed.
+
+(* The footprint contained in the location of a place *)
+Lemma eval_place_sound: forall e m p b ofs own fpm (* init uninit universe *)
+    (EVAL: eval_place ce e m p b ofs)
+    (MM: mmatch fpm ce m e own)
+    (WFOWN: wf_env fpm ce m e)
+    (WT: wt_place (env_to_tenv e) ce p)
+    (* (SOWN: sound_own own init uninit universe) *)
+    (* evaluating the address of p does not require that p is
+    owned. Shallow own is used in bmatch *)
+    (POWN: dominators_is_init (* init uninit universe *) own p = true),
+  exists fp (* ce' *) (* phl *),
+    get_loc_footprint_map e (path_of_place p) fpm = Some (b, (Ptrofs.unsigned ofs), fp)
+    /\ wt_footprint ce (typeof_place p) fp
+    (* range *)
+    /\ (Ptrofs.unsigned ofs) + (sizeof ce (typeof_place p)) <= Ptrofs.max_unsigned
+    (* we need to consider the assignment to this place *)
+    /\ Mem.range_perm m b (Ptrofs.unsigned ofs) (Ptrofs.unsigned ofs + sizeof ce (typeof_place p)) Cur Freeable
+    (* range_perm cannot guarantee that b is a valid block *)
+    /\ Mem.valid_block m b
+.
+Proof.
+  induction 1; intros.
+  (* Plocal *)
+  - rewrite Ptrofs.unsigned_zero.
+    exploit wf_env_footprint; eauto. intros (fp & FP & WTFP).
+    exists fp. repeat apply conj. simpl. rewrite H. rewrite FP. auto.
+    simpl. auto.
+    simpl. eapply sizeof_in_range. inv WT. auto.
+    eapply wf_env_freeable; eauto.
+    eapply wf_env_freeable; eauto.    
+  (* Pfield *)
+  - inv WT.
+    (* two type facts, reduce one *)
+    rewrite H in WT2. inv WT2. rewrite H0 in WT3. inv WT3.
+    exploit IHEVAL. 1-5: auto.
+    intros (fp & PFP & WTFP & RAN0 & FREE). rewrite H in RAN0. simpl in RAN0.
+    (** Inversion of WTFP *)
+    rewrite H in WTFP. inv WTFP; simpl in *; try congruence.
+    rewrite H0 in *. inv CO.
+    exploit WT0; eauto. intros (ffp & fofs & INFPL & FOFS& WTFP1).
+    (* construct some range hypotheses *)
+    exploit field_offset_in_max_range; eauto.
+    intros (R1 & R2 & R3). 
+    rewrite H1 in FOFS. inv FOFS. 
+    (* exploit field_type_implies_field_tag; eauto. intros (tag & FTAG & TAGN). *)
+    erewrite Ptrofs.add_unsigned.
+    rewrite Ptrofs.unsigned_repr. 1-2: rewrite Ptrofs.unsigned_repr; auto.
+    exists ffp. repeat apply conj; auto.
+    (* get_loc_footprint_map *)
+    simpl. destruct (path_of_place p) eqn: POP.
+    eapply get_loc_footprint_map_app. eauto.
+    simpl.  rewrite INFPL. auto.
+    (* permission *)
+    exploit field_offset_in_range_complete; eauto.
+    intros R4.
+    red. intros. eapply FREE. rewrite H. simpl.
+    rewrite H0. lia.
+    (* valid_block *)
+    eapply FREE.
+  (* Pdowncast *)
+  - inv WT.
+    rewrite H in WT2. inv WT2. rewrite H0 in WT3. inv WT3.
+    (** TODO: make it a lemma: prove p's dominators are init *)
+    (** It is impossible to be proved  *)
+    assert (PDOM: dominators_is_init (* init uninit universe *) own p = true).
+    { unfold dominators_is_init in *. simpl in *.
+      eapply andb_true_iff in POWN. destruct POWN as (A & B).
+      destruct p; simpl in *; auto.
+      eapply andb_true_iff. auto. }
+    (** Prove that p is_init  *)
+    exploit IHEVAL. 1-5: auto.
+    intros (fp & PFP & WTFP & RAN0 & PERM).
+    rewrite H in RAN0. simpl in RAN0. rewrite H0 in RAN0.
+    (* construct some range hypotheses *)
+    exploit variant_field_offset_in_max_range; eauto.
+    intros (R1 & R2 & R3). 
+    (* produce some range requirement *)
+    erewrite Ptrofs.add_unsigned.
+    rewrite Ptrofs.unsigned_repr. 1-2: rewrite Ptrofs.unsigned_repr; auto.
+    (** Prove that p is_init: NO!! We can only show that (valid_owner
+    p) is init *)
+    exploit valid_owner_place_footprint. eauto. eauto. intros (fp1 & ofs1 & fofs1 & PFP1 & VOFS1 & OFSEQ).
+    unfold dominators_must_init in POWN. simpl in POWN.
+    eapply andb_true_iff in POWN. destruct POWN as (PINIT & POWN).
+    exploit MM. eauto. auto.
+    (* valid owner's bmatch implies subfield bmatch *)
+    intros (BM & FULL).
+    assert (BM1: bmatch ce m b (Ptrofs.unsigned ofs) fp).
+    { rewrite OFSEQ. eapply valid_owner_bmatch. eauto. eauto. }
+    rewrite H in WTFP. (* inv BM1. *)
+    (* rewrite some redundant premises *)
+    simpl in H1. 
+    inv WTFP; simpl in *; try congruence. inv BM1.
+    inv BM1. rewrite H1 in TAG0. inv TAG0. rewrite Int.unsigned_repr in H2.
+    (* do some rewrting *)
+    rewrite H0 in CO. inv CO.
+    rewrite H2 in TAG. inv TAG. simpl.
+    rewrite H3 in FOFS. inv FOFS.
+    exists fp0. repeat apply conj.
+    (* get_loc_footprint_map *)
+    destruct (path_of_place p) eqn: POP.
+    eapply get_loc_footprint_map_app. eauto. simpl.
+    rewrite H. repeat destruct ident_eq; simpl; try congruence.
+    destruct list_eq_dec; simpl; try congruence.
+    auto.
+    lia.
+    (* permission *)
+    rewrite H in PERM. simpl in PERM. rewrite H0 in PERM.
+    exploit variant_field_offset_in_range_complete; eauto.
+    intros (R4 & R5). red. intros. eapply PERM. lia.
+    eapply PERM.
+    generalize (list_nth_z_range _ _ TAG).
+    generalize (COMP_LEN id0 co CO). 
+    lia.
+  (* Pderef *)
+  - inv WT.
+    unfold dominators_must_init in POWN. simpl in POWN.
+    eapply andb_true_iff in POWN. destruct POWN as (PINIT & POWN).    
+    exploit IHEVAL; eauto.
+    intros (fp & PFP & WTFP & RAN0 & PERM).
+    exploit MM. eauto. auto.
+    intros (BM & FULL). destruct (typeof_place p) eqn: PTY; simpl in WT2; try congruence.
+    inv WT2.
+    inv WTFP; inv BM; simpl in *; try congruence.
+    exists fp0. repeat apply conj.    
+    (* prove ofs' = 0 *)
+    inv H; simpl in *; try congruence.
+    simpl in *. inv H0. rewrite LOAD in H1. inv H1.
+    rewrite Ptrofs.unsigned_zero.    
+    (* get_loc_footprint_map *)
+    destruct (path_of_place p) eqn: POP.
+    eapply get_loc_footprint_map_app. eauto.
+    simpl. auto.
+    (* wt_footprint *)
+    simpl. auto.
+    (* range proof: first show that ofs' is zero *)
+    inv H; simpl in *; try congruence.
+    inv H0. rewrite LOAD in H1. inv H1. rewrite Ptrofs.unsigned_zero.
+    lia.
+    (* permission *)
+    inv H; simpl in *; try congruence.
+    inv H0. rewrite LOAD in H1. inv H1.
+    red. intros. eapply VRES.
+    generalize (size_chunk_pos Mptr).
+    rewrite Ptrofs.unsigned_zero in H. lia.
+    inv H; simpl in *; try congruence.
+    inv H0. rewrite LOAD in H1. inv H1.
+    (* valid_block *)
+    eapply Mem.valid_access_valid_block.
+    eapply Mem.valid_access_implies. eapply Mem.load_valid_access. eauto.
+    constructor.
+Qed.
+
+(* The location of the member is sem_wt_loc. It is used in the invariant of dropstate *)
+Inductive member_footprint (m: mem) (co: composite) (b: block) (ofs: Z) (fp: footprint) : member -> Prop :=
+| member_footprint_struct: forall fofs fid fty
+    (STRUCT: co.(co_sv) = Struct)
+    (FOFS: field_offset ce fid co.(co_members) = OK fofs)
+    (FTY: field_type fid co.(co_members) = OK fty)
+    (WTLOC: sem_wt_loc ce m fp b (ofs + fofs))
+    (WTFP: wt_footprint ce fty fp),
+    member_footprint m co b ofs fp (Member_plain fid fty)
+.
+
+(* hacking: simulate the deref_loc_rec to get the path, footprint and
+location of the value. fp is the start of the footprint. *)
+Inductive deref_loc_rec_footprint (m: mem) (b: block) (ofs: Z) (fty: type) (fp: footprint) : list type -> block -> Z -> type -> footprint -> Prop :=
+| deref_loc_rec_footprint_nil:
+  deref_loc_rec_footprint m b ofs fty fp nil b ofs fty fp
+| deref_loc_rec_footprint_cons: forall ty tys fp2 b1 ofs1 b2 sz
+    (* simulate type_to_drop_member_state *)
+    (DEREF: deref_loc_rec_footprint m b ofs fty fp tys b1 ofs1 (Tbox ty) (fp_box b2 sz fp2))
+    (TYSZ: sz = sizeof ce ty)
+    (* Properties of bmatch *)
+    (LOAD: Mem.load Mptr m b1 ofs1 = Some (Vptr b2 Ptrofs.zero))
+    (SIZE: Mem.load Mptr m b2 (- size_chunk Mptr) = Some (Vptrofs (Ptrofs.repr sz)))
+    (PERM: Mem.range_perm m b2 (- size_chunk Mptr) sz Cur Freeable)
+    (RANGE: 0 < sz <= Ptrofs.max_unsigned),
+    deref_loc_rec_footprint m b ofs fty fp ((Tbox ty) :: tys) b2 0 ty fp2.
+
+
+(** TODO  *)
+Inductive drop_member_footprint (m: mem) (co: composite) (b: block) (ofs: Z) (fp: footprint) : option drop_member_state -> Prop :=.
+
+
+(** TODO  *)
+Inductive sound_drop_place_state (e: env) (m: mem) (fpm: fp_map) (own: own_env) : footprint -> option drop_place_state -> Prop :=.
+
+(* soundness of continuation: the execution of current function cannot
+modify the footprint maintained by the continuation *)
+
+
+Inductive sound_cont : INIT_AN -> LOANS_AN -> statement -> rustcfg -> cont -> cfg_kinfo -> mem -> fp_frame -> Prop :=
+| sound_Kstop: forall init_an loans_an body cfg nret m
+    (RET: cfg ! nret = Some Iend),
+    sound_cont init_an loans_an body cfg Kstop (mk_cfg_kinfo nret None None nret) m fpf_emp
+| sound_Kseq: forall init_an loans_an body cfg s ts k pc next cont brk nret m fpf
+    (MSTMT: move_check_stmt init_an body cfg s ts (mk_cfg_info pc next cont brk nret))
+    (MCONT: sound_cont init_an loans_an body cfg k (mk_cfg_kinfo next cont brk nret) m fpf),
+    sound_cont init_an loans_an body cfg (Kseq s k) (mk_cfg_kinfo pc cont brk nret) m fpf
+| sound_Kloop: forall init_an loans_an body cfg s ts k body_start loop_jump_node exit_loop nret contn brk m fpf
+    (START: cfg ! loop_jump_node = Some (Inop body_start))
+    (MSTMT: move_check_stmt init_an body cfg s ts (mk_cfg_info body_start loop_jump_node (Some loop_jump_node) (Some exit_loop) nret))
+    (MCONT: sound_cont init_an loans_an body cfg k (mk_cfg_kinfo exit_loop contn brk nret) m fpf),
+    sound_cont init_an loans_an body cfg (Kloop s k) (mk_cfg_kinfo loop_jump_node (Some loop_jump_node) (Some exit_loop) nret) m fpf
+| sound_Kcall: forall init_an loans_an body cfg k nret f e own p m fpf
+    (MSTK: sound_stacks (Kcall p f e own k) m fpf)
+    (RET: cfg ! nret = Some Iend)
+    (WFOWN: wf_own_env e ce own),
+    sound_cont init_an loans_an body cfg (Kcall p f e own k) (mk_cfg_kinfo nret None None nret) m fpf
+| sound_Kdropplace: forall f st ps nret cfg pc cont brk k own1 own2 e m maybeInit maybeUninit universe entry fpm fpf mayinit mayuninit rfp  live loans_env
+    (INITAN: InitAnalysis.analyze ce f cfg entry = OK (maybeInit, maybeUninit, universe))   
+    (LOANSAN: loans_flow_analyze ce f cfg entry = OK (live, loans_env))
+    (MCONT: sound_cont (maybeInit, maybeUninit, universe) (live, loans_env) f.(fn_body) cfg k (mk_cfg_kinfo pc cont brk nret) m fpf)
+    (MM: mmatch fpm ce m e own1)
+    (WFNEV: wf_env fpm ce m e)
+    (** VERY DIFFICULT: Invariant of drop_place_state *)
+    (SDP: sound_drop_place_state e m fpm own1 rfp st)
+    (SEP: list_norepet (flat_fp_frame (fpf_dropplace e fpm rfp fpf)))
+    (MOVESPLIT: move_split_places own1 ps = own2)
+    (* ordered property of the split places used to prove sound_state after the dropplace *)
+    (ORDERED: move_ordered_split_places_spec own1 (map fst ps))
+    (* all places in drops are wt_place *)
+    (WTPS: Forall (fun p => wt_place e ge p) (map fst ps))
+    (IM: get_IM_state maybeInit!!pc maybeUninit!!pc (Some (mayinit, mayuninit)))
+    (OWN: sound_own own2 mayinit mayuninit universe)
+    (WFOWN: wf_own_env e ce own1)
+    (FULL: (forall p full, In (p, full) ps -> is_full (own_universe own1) p = full))
+    (* (WTRFP: wt_footprint ce rfpty rfp) *),
+    sound_cont (maybeInit, maybeUninit, universe) (live, loans_env) f.(fn_body) cfg (Kdropplace f st ps e own1 k) (mk_cfg_kinfo pc cont brk nret) m (fpf_dropplace e fpm rfp fpf)
+| sound_Kdropcall: forall init_an loans_an body cfg k pc cont brk nret fpf st co fp ofs b membs fpl id m
+    (CO: ce ! id = Some co)
+    (DROPMEMB: drop_member_footprint m co b (Ptrofs.unsigned ofs) fp st)
+    (MEMBFP: list_forall2 (member_footprint m co b (Ptrofs.unsigned ofs)) fpl membs)
+    (RANGE: Ptrofs.unsigned ofs + co_sizeof co <= Ptrofs.max_unsigned)
+    (** Do we need some separation properties? *)
+    (SOUND: sound_cont init_an loans_an body cfg k (mk_cfg_kinfo pc cont brk nret) m fpf)
+    (INFRM: In b (flat_fp_frame fpf))
+    (CONTDIS: ~ In b (footprint_flat fp ++ flat_map footprint_flat fpl)),
+    sound_cont init_an loans_an body cfg (Kdropcall id (Vptr b ofs) st membs k) (mk_cfg_kinfo pc cont brk nret) m (fpf_drop fp fpl fpf)
+
+with sound_stacks : cont -> mem -> fp_frame -> Prop :=
+| sound_stacks_stop: forall m,
+    sound_stacks Kstop m fpf_emp
+| sound_stacks_call: forall f nret cfg pc contn brk k own1 own2 p e m maybeInit maybeUninit universe entry fpm fpf mayinit mayuninit live loans_env
+    (INITAN: InitAnalysis.analyze ce f cfg entry = OK (maybeInit, maybeUninit, universe))   
+    (LOANSAN: loans_flow_analyze ce f cfg entry = OK (live, loans_env))
+    (MCONT: sound_cont (maybeInit, maybeUninit, universe) (live, loans_env) f.(fn_body) cfg k (mk_cfg_kinfo pc contn brk nret) m fpf)
+    (MM: mmatch fpm ce m e own1)
+    (WFENV: wf_env fpm ce m e)
+    (* we need to maintain this invariant for p's evaluation when
+    function return *)
+    (DOM: dominators_is_init own1 p = true)
+    (* own2 is built after the function call *)
+    (AFTER: own2 = init_place own1 p)
+    (IM: get_IM_state maybeInit!!pc maybeUninit!!pc (Some (mayinit, mayuninit)))
+    (OWN: sound_own own2 mayinit mayuninit universe)
+    (WFOWN: wf_own_env e ce own1),
+    sound_stacks (Kcall p f e own1 k) m (fpf_func e fpm fpf).
+    
+
+(** TODO: invariant for the borrow checking  *)
+Inductive sound_state: state -> Prop :=
+| sound_regular_state: forall f cfg entry maybeInit maybeUninit universe s ts pc next cont brk nret k e own m fpm fpf flat_fp sg mayinit mayuninit Hm live loans_env bor_stk
+    (INITAN: InitAnalysis.analyze ce f cfg entry = OK (maybeInit, maybeUninit, universe))   
+    (LOANSAN: loans_flow_analyze ce f cfg entry = OK (live, loans_env))
+    (MCK_STMT: move_check_stmt (maybeInit, maybeUninit, universe) f.(fn_body) cfg s ts (mk_cfg_info pc next cont brk nret))
+    (CONT: sound_cont (maybeInit, maybeUninit, universe) (live, loans_env) f.(fn_body) cfg k (mk_cfg_kinfo next cont brk nret) m fpf)
+    (IM: get_IM_state maybeInit!!pc maybeUninit!!pc (Some (mayinit, mayuninit)))
+    (OWN: sound_own own mayinit mayuninit universe)
+    (MM: mmatch fpm ce m e own)
+    (FLAT: flat_fp = flat_fp_frame (fpf_func e fpm fpf))
+    (* footprint is separated *)
+    (NOREP: list_norepet flat_fp)
+    (ACC: rsw_acc w (rsw sg flat_fp m Hm))
+    (* we need to maintain the well-formed invariant of own_env *)
+    (WFENV: wf_env fpm ce m e)
+    (* invariant of the own_env *)
+    (WFOWN: wf_own_env e ce own),
+    sound_state (State f s k e own bor_stk m)
+| sound_dropplace: forall f cfg entry maybeInit maybeUninit universe next cont brk nret st drops k e own1 own2 m fpm fpf flat_fp sg mayinit mayuninit rfp Hm live loans_env bor_stk
+    (INITAN: InitAnalysis.analyze ce f cfg entry = OK (maybeInit, maybeUninit, universe))   
+    (LOANSAN: loans_flow_analyze ce f cfg entry = OK (live, loans_env))
+    (CONT: sound_cont (maybeInit, maybeUninit, universe) (live, loans_env) f.(fn_body) cfg k (mk_cfg_kinfo next cont brk nret) m fpf)
+    (MM: mmatch fpm ce m e own1)
+    (FLAT: flat_fp = flat_fp_frame (fpf_dropplace e fpm rfp fpf))
+    (NOREP: list_norepet flat_fp)
+    (ACC: rsw_acc w (rsw sg flat_fp m Hm))
+    (* every place in the drop_fully_owned state is owned: this may be
+    wrong because it does not consider own is changing *)
+    (SDP: sound_drop_place_state e m fpm own1 rfp st)
+    (* big step update of the own_env *)
+    (MOVESPLIT: move_split_places own1 drops = own2)
+    (* ordered property of the split places used to prove sound_state after the dropplace *)
+    (ORDERED: move_ordered_split_places_spec own1 (map fst drops))
+    (* fullspec is used to maintain the invariant between is_full and the full flags *)
+    (FULLSPEC: forall p full,  In (p, full) drops -> is_full (own_universe own1) p = full)
+    (* all places in drops are wt_place *)
+    (WTPS: Forall (fun p => wt_place e ge p) (map fst drops))
+    (WF: wf_env fpm ce m e)
+    (* We just want to make rfp well structured (e.g., field names are
+    norepet and the size of blocks are in range) *)
+    (* (WTRFP: wt_footprint ce rfpty rfp)  *)
+    (IM: get_IM_state maybeInit!!next maybeUninit!!next (Some (mayinit, mayuninit)))
+    (* Why sound_own own2 here not own1? because the analysis result is about the next node *)
+    (OWN: sound_own own2 mayinit mayuninit universe)
+    (WFOWN: wf_own_env e ce own1),
+    (* no need to maintain borrow check domain in dropplace? But how
+    to record the pc and next statement? *)
+    sound_state (Dropplace f st drops k e own1 bor_stk m)
+| sound_dropstate: forall init_an loans_an body cfg next cont brk nret id co fp fpl b ofs st m membs k fpf flat_fp sg Hm bor_stk
+    (CO: ce ! id = Some co)
+    (* The key is how to prove semantics well typed can derive the
+    following two properties *)
+    (DROPMEMB: drop_member_footprint m co b (Ptrofs.unsigned ofs) fp st)
+    (* all the remaining members are semantically well typed *)
+    (MEMBFP: list_forall2 (member_footprint m co b (Ptrofs.unsigned ofs)) fpl membs)
+    (CONT: sound_cont init_an loans_an body cfg k (mk_cfg_kinfo next cont brk nret) m fpf)
+    (FLAT: flat_fp = flat_fp_frame (fpf_drop fp fpl fpf))
+    (NOREP: list_norepet flat_fp)
+    (* The location of the composite to be dropped is not in the
+    current footprint ! Note that it may resides in fpf! *)
+    (DIS: ~ In b (footprint_flat fp ++ flat_map footprint_flat fpl))
+    (* b is in fpf to make sure that changing the memory outside
+    flat_fp does not change b *)
+    (INFRM: In b (flat_fp_frame fpf))
+    (ACC: rsw_acc w (rsw sg flat_fp m Hm))
+    (RANGE: Ptrofs.unsigned ofs + co_sizeof co <= Ptrofs.max_unsigned),
+    sound_state (Dropstate id (Vptr b ofs) st membs k bor_stk m)
+| sound_callstate: forall vf fd orgs org_rels tyargs tyres cconv m fpl args fpf k flat_fp sg Hm bor_stk
+    (FUNC: Genv.find_funct ge vf = Some fd)
+    (FUNTY: type_of_fundef fd = Tfunction orgs org_rels tyargs tyres cconv)
+    (* arguments are semantics well typed *)
+    (WTVAL: list_forall2 (sem_wt_val ce m) fpl args)
+    (* Used in assign_loc_sound in function entry proof *)
+    (ANORM: val_casted_list args tyargs)
+    (WTFP: list_forall2 (wt_footprint ce) (type_list_of_typelist tyargs) fpl)
+    (STK: sound_stacks k m fpf)
+    (FLAT: flat_fp = flat_fp_frame fpf ++ flat_map footprint_flat fpl)
+    (* also disjointness of fpl and fpf *)
+    (NOREP: list_norepet flat_fp)
+    (ACC: rsw_acc w (rsw sg flat_fp m Hm)),
+    sound_state (Callstate vf args k bor_stk m)
+| sound_returnstate: forall sg fpf flat_fp m k retty rfp v Hm bor_stk
+    (* For now, all function must have return type *)
+    (RETY: typeof_cont_call (rs_sig_res sg) k = retty)
+    (WTVAL: sem_wt_val ce m rfp v)
+    (CAST: val_casted v retty)
+    (WTFP: wt_footprint ce retty rfp)
+    (FLAT: flat_fp = footprint_flat rfp ++ flat_fp_frame fpf)
+    (SEP: list_norepet flat_fp)
+    (STK: sound_stacks k m fpf)
+    (ACC: rsw_acc w (rsw sg flat_fp m Hm)),
+    sound_state (Returnstate v k bor_stk m)
+.
+
+
+
+End BORROW_CHECK.
+
+
+(** TODO: the interface for the borrow checking *)
+Definition rs_bor : invariant li_rs_bor := inv_bot.
+
+Definition own2bor (I: invariant li_rs) : invariant li_rs_bor :=
+  {| inv_world := inv_world I;
+    symtbl_inv := symtbl_inv I;
+    query_inv w (q: query li_rs_bor) := (query_inv I w q);
+    reply_inv w (r: reply li_rs_bor) := (reply_inv I w r); |}.
+
+(* Given a module [M], if it passes the borrow checking and it does
+not contain errors except for memory errors at its source semantics,
+then its stacked borrow semantics (which is defined by adding stacked
+borrow rules to the original RustIR semanitcs) has no undefined
+behavior. As our semantics are open, we should specify the
+rely-guarantee conditions at the module boundaries to restrict the
+interference with the unknown environment. We use the interface
+[rs_bor] to represent this condition. *)
+Lemma borrow_check_soundness_stacked_borrow (P Q: invariant li_rs) (M M': RustIR.program) :
+  module_type_safe P Q (RustIRown.semantics M) (RustIRown.mem_error M) ->  
+  borrow_check_program M = OK M' ->
+  module_type_safe ((own2bor P) @@ rs_bor) ((own2bor Q) @@ rs_bor) (RustIRbor.semantics M) SIF.
+Proof.
+Admitted.
+
+
+Definition rs_bor1 : invariant li_rs :=
+  {| inv_world := inv_world rs_bor;
+    symtbl_inv := symtbl_inv rs_bor;
+    query_inv w (q: query li_rs) := exists stk, query_inv rs_bor w (rsbor_q q stk);
+    reply_inv w (r: reply li_rs) := exists stk, reply_inv rs_bor w (rsbor_r r stk) |}.
+
+(* When module [M] has no UB in the stacked borrow semantics, it also
+has no UB in the orignal semantics, under the interface [rs_bor1 q :=
+exists stk, rs_bor (q, stk)]. *)
+Theorem borrow_check_safe (P Q: invariant li_rs) (M M': RustIR.program) :
+  module_type_safe P Q (RustIRown.semantics M) (RustIRown.mem_error M) ->  
+  borrow_check_program M = OK M' ->
+  module_type_safe (P @@ rs_bor1) (Q @@ rs_bor1) (RustIRown.semantics M) SIF.
+Proof.
+Admitted.
