rustfrontend/Listmisc.v
@@ -1,0 +1,96 @@
+Require Import Coqlib.
+Require Import AST.
+
+Import ListNotations.
+
+(** find an element from list  *)
+
+Fixpoint list_find {A} (f : A -> bool) (l: list A) : option (nat * A) :=  
+  match l with
+  | nil => None
+  | x :: l => if f x then Some (O,x) else option_map (fun '(idx, elt) => (S idx, elt)) (list_find f l)
+  end.
+
+Lemma list_find_some : forall (A: Type) (l: list A) f a idx,
+    list_find f l = Some (idx, a) ->
+    nth_error l idx = Some a /\ f a = true.
+Admitted.
+
+
+Lemma list_find_none : forall (A: Type) (l: list A) f,
+    list_find f l = None ->
+    forall x, In x l -> f x = false.
+Admitted.
+
+
+(* find an element with ident as the key *)
+
+Definition find_field {A: Type} (id: ident) (l: list (ident * A)) : option A :=
+  option_map (fun '(idx, (id, a)) => a) (list_find (fun '(id', _) => if ident_eq id id' then true else false) l). 
+
+
+Lemma find_field_some: forall (A: Type) fid fpl (a: A),
+    find_field fid fpl = Some a ->
+    In (fid, a) fpl.
+Proof.
+  intros. unfold find_field in H.
+  destruct (list_find (fun '(id', _) => if ident_eq fid id' then true else false) fpl) eqn: FIND; inv H.
+  destruct p.
+  exploit list_find_some. eauto. intros (A1 & B).
+  destruct p.
+  destruct ident_eq in B; try congruence.
+  subst. eapply nth_error_in. eauto.
+Qed.
+
+Definition field_idents {A: Type} (l: list (ident * A)) : list ident :=
+  map (fun '(fid, _) => fid) l.
+
+(* only set the first occurence of fid *)
+Fixpoint set_field {A: Type} (id: ident) (f: A -> A) (l: list (ident * A)) : list (ident * A) :=
+  match l with
+  | nil => nil
+  | (id', a') :: l' =>
+      if ident_eq id id' then
+        (id, f a') :: l'
+      else
+        (id', a') :: (set_field id f l')
+  end.
+
+(* Properties for find_field and set_field *)
+
+Lemma find_field_split : forall A fpl id (a:A),
+    find_field id fpl = Some a ->
+    exists l1 l2,
+      fpl = l1 ++ (id, a) :: l2
+      /\ ~ In id (field_idents l1).
+Proof.
+  induction fpl; simpl; intros.
+  - inv H.
+  - destruct a. unfold find_field in H.
+    destruct ((list_find (fun '(id', _) => if ident_eq id id' then true else false)
+             ((i, a) :: fpl))) eqn: FIND; inv H.
+    simpl in FIND.
+    destruct ident_eq in FIND.
+    + inv FIND. exists nil, fpl.
+      split. simpl. auto.
+      intro. inv H.
+    + destruct (list_find (fun '(id', _) => if ident_eq id id' then true else false)) eqn: FIND1; inv FIND.
+      destruct p0 as (i1 & (i2 & a3)).
+      exploit IHfpl. 
+      unfold find_field. rewrite FIND1. reflexivity.
+      intros (l1 & l2 & A1 & A2).
+      subst.
+      exists ((i,a)::l1), l2. split; auto.
+      intro. inv H; congruence. 
+Qed.
+      
+Lemma set_field_split : forall A l1 l2 id f (a: A),
+    ~ In id (field_idents l1) ->
+    set_field id f (l1 ++ (id, a) :: l2) = (l1 ++ (id, f a) :: l2).
+Proof.
+  induction l1; simpl; intros.
+  - destruct ident_eq; try congruence.
+  - destruct a. eapply Decidable.not_or in H.
+    destruct H. destruct ident_eq; try congruence.
+    f_equal. eauto.
+Qed.
