Makefile
@@ -178,6 +178,7 @@ RUSTFRONTEND=Rusttypes.v Rustsyntax.v Rustlight.v RustIR.v\
   StkBorPermission.v RustIRbor.v\
   BorrowCheckDomain.v ReplaceOrigins.v BorrowCheckPolonius.v\
   RegionLiveness.v BorrowCheck.v BorrowCheckSound.v\
+  Listmisc.v\
   # BorrowCheckSafe.v
 
 # RUSTDEMO=LinkedList.v LinkedListSafe.v HashMap.v HashMapSafe.v HashMapCommon.v \
